src/reordering/ReordExecNaNb.v
@@ -501,7 +501,7 @@ Proof using INV INV'.
     { now rewrite rsr_mappero. }
     destruct (BINRW b_t) as [RR | WW]; vauto.
     { apply XmmCons.read_extent with (G_t := G_t')
-        (sc_t := WCore.sc X_t') (a := b_t) (m := mapper); eauto.
+        (a := b_t) (m := mapper); eauto.
       { apply SIMREL'. }
       { rewrite (rsr_acts SIMREL').
         rewrite extra_a_some; auto with hahn.
@@ -549,7 +549,7 @@ Proof using INV INV'.
       apply G_s_wf with (X_t := X_t') (a_t := a_t)
                 (b_t := b_t) (mapper := mapper); vauto. }
     apply XmmCons.write_extent with (G_t := G_t')
-      (sc_t := WCore.sc X_t') (a := b_t) (m := mapper); eauto.
+      (a := b_t) (m := mapper); eauto.
     { apply SIMREL'. }
     { rewrite (rsr_acts SIMREL').
       rewrite extra_a_some; auto with hahn.
@@ -627,10 +627,12 @@ Proof using INV INV'.
             cross_false_l, cross_false_r.
     now rewrite !union_false_r. }
   apply XmmCons.monoton_cons with (G_t := G_t')
-              (sc_t := WCore.sc X_t') (m := mapper); eauto.
+              (m := mapper); eauto.
   all: try now apply SIMREL'.
   { now rewrite (rsr_acts SIMREL'), EXTRA, set_union_empty_r. }
   { rewrite (rsr_rf SIMREL'), EXTRA. basic_solver 8. }
+  { rewrite (rsr_co SIMREL'), EXTRA.
+    now rewrite set_inter_empty_l, add_max_empty_r, union_false_r. }
   eapply G_s_wf with (X_t := X_t'); eauto.
 Admitted.
 
